\documentclass[]{article}
%made from template named MathArticleTemplate
\usepackage{amsfonts}
\usepackage{amsmath}
\usepackage{amsthm}
\usepackage{amssymb}
\usepackage{hyperref}
\hypersetup{colorlinks=true}
\usepackage{graphics}

%Fix \eqref in section title
\pdfstringdefDisableCommands{\def\eqref#1{(\ref{#1})}}

\DeclareMathOperator{\es}{Es}
\DeclareMathOperator{\ez}{Ez}
\DeclareMathOperator{\gs}{gs}
\DeclareMathOperator{\md}{mod}
\DeclareMathOperator{\pow}{Pow}
%Parenthesis, Braces, Brackets usepackage{physics}
\newcommand{\pqty}[1]{{\left(#1\right)}}
\newcommand{\Bqty}[1]{{\left\{#1\right\}}}
\newcommand{\bqty}[1]{{\left[#1\right]}}
\newcommand{\abs}[1]{{\left\lvert#1\right\rvert}}
%other stuff
\newcommand{\floor}[1]{{\left\lfloor#1\right\rfloor}}
\newcommand{\ceil}[1]{{\left\lceil#1\right\rceil}}
%Laplace transform and inverse
\newcommand{\laplace}[1]{\mathcal{L}\Bqty{#1}\pqty{s}}
\newcommand{\laplaceInv}[1]{\mathcal{L}^{-1}\Bqty{#1}\pqty{t}}
%Derivatives
\newcommand{\pdiff}[2]{\frac{\partial^{#2}}{\partial #1^{#2}}}

%lemma,theorem, proof
\newtheorem{theorem}{Theorem}[section]
\newtheorem{lemma}[theorem]{Lemma}
\newtheorem{definition}[theorem]{Definition}
\newtheorem{corollary}[theorem]{Corollary}

\numberwithin{equation}{section}

\usepackage{xr}
\externaldocument{Logarithms}

%\usepackage{minted}
%opening
\author{Mark Andrew Gerads: nazgand@gmail.com}

\title{Differentiation}

\begin{document}
	
	\maketitle
	
	\begin{abstract}
		The goal of this paper is to review differentiation.
	\end{abstract}
	
	\section{Definition}
	\begin{equation}
	\label{DerivLimit}
	\pdiff{x}{}f\pqty{x}=\lim\limits_{h\to 0}\frac{f\pqty{x+h}-f\pqty{x}}{h}
	\end{equation}
	
	\section{Sum Rule}
	\begin{theorem}
		\begin{equation}
		\label{DiffSum}
		\pdiff{x}{}\pqty{f\pqty{x}+g\pqty{x}}=
		\pqty{\pdiff{x}{}f\pqty{x}}+
		\pqty{\pdiff{x}{}g\pqty{x}}
		\end{equation}
	\end{theorem}
	\begin{proof}
		Use \eqref{DerivLimit}
		\begin{equation}
		\pdiff{x}{}\pqty{f\pqty{x}+g\pqty{x}}
		=\lim\limits_{h\to 0}
		\frac{\pqty{f\pqty{x+h}+g\pqty{x+h}}-\pqty{f\pqty{x}+g\pqty{x}}}{h}
		\end{equation}
		Rearrange
		\begin{equation}
		\pdiff{x}{}\pqty{f\pqty{x}+g\pqty{x}}
		=\lim\limits_{h\to 0}
		\pqty{\frac{{f\pqty{x+h}-f\pqty{x}}}{h}
		+
		\frac{{g\pqty{x+h}-g\pqty{x}}}{h}}
		\end{equation}
		Split the limit
		\begin{equation}
		\pdiff{x}{}\pqty{f\pqty{x}+g\pqty{x}}
		=\pqty{\lim\limits_{h\to 0}
		\frac{{f\pqty{x+h}-f\pqty{x}}}{h}}
			+ \pqty{\lim\limits_{a\to 0}
			\frac{{g\pqty{x+a}-g\pqty{x}}}{a}}
		\end{equation}
		Simplify with \eqref{DerivLimit}
		\begin{equation}
		\pdiff{x}{}\pqty{f\pqty{x}+g\pqty{x}}=
		\pqty{\pdiff{x}{}f\pqty{x}}+
		\pqty{\pdiff{x}{}g\pqty{x}}
		\end{equation}
	\end{proof}

	\section{Constant Multiple Rule}
	\begin{theorem}
		\begin{equation}
			\pdiff{x}{}\pqty{a*f\pqty{x}}=
			a*\pdiff{x}{}\pqty{f\pqty{x}}
		\end{equation}
	\end{theorem}
	\begin{proof}
		Use \eqref{DerivLimit}
		\begin{equation}
		\pdiff{x}{}\pqty{a*f\pqty{x}}=
		\lim\limits_{h\to 0}\frac{a*f\pqty{x+h}-a*f\pqty{x}}{h}=
		a*\lim\limits_{h\to 0}\frac{f\pqty{x+h}-f\pqty{x}}{h}=
		a*\pdiff{x}{}\pqty{f\pqty{x}}
		\end{equation}
	\end{proof}
	
	\section{Chain Rule}
	\begin{theorem}
		\begin{equation}
		\label{DiffChainRule}
		\pdiff{x}{}{f\pqty{g\pqty{x}}}
		=\pqty{\pdiff{g}{}f\pqty{g}:g\to g\pqty{x}}*\pdiff{x}{}{g\pqty{x}}
		\end{equation}
	\end{theorem}
	\begin{proof}
		Start with \eqref{DerivLimit}
		\begin{equation}
		\pdiff{x}{}{f\pqty{g\pqty{x}}}
		=\lim\limits_{h\to 0}
		\frac{f\pqty{g\pqty{x+h}}-f\pqty{g\pqty{x}}}{h}
		\end{equation}
		Multiply by \(1=\frac{g\pqty{x+h}-g\pqty{x}}{g\pqty{x+h}-g\pqty{x}}\):
		\begin{equation}
		\pdiff{x}{}{f\pqty{g\pqty{x}}}
		=\lim\limits_{h\to 0}
		\frac{f\pqty{g\pqty{x+h}}-f\pqty{g\pqty{x}}}{g\pqty{x+h}-g\pqty{x}}
		\frac{g\pqty{x+h}-g\pqty{x}}{h}
		\end{equation}
		Split the limit:
		\begin{equation}
		\pdiff{x}{}{f\pqty{g\pqty{x}}}
		=\lim\limits_{h\to 0}
		\frac{f\pqty{g\pqty{x+h}}-f\pqty{g\pqty{x}}}{g\pqty{x+h}-g\pqty{x}}
		\lim\limits_{a\to 0}
		\frac{g\pqty{x+a}-g\pqty{x}}{a}
		\end{equation}
		Simplify \eqref{DerivLimit}
		\begin{equation}
		\pdiff{x}{}{f\pqty{g\pqty{x}}}
		=\lim\limits_{h\to 0}
		\frac{f\pqty{g\pqty{x+h}}-f\pqty{g\pqty{x}}}{g\pqty{x+h}-g\pqty{x}}
		\pdiff{x}{}{g\pqty{x}}
		\end{equation}
		Substitute \(g\pqty{x+h}\to g+\epsilon,g\pqty{x}\to g\)
		\begin{equation}
		\pdiff{x}{}{f\pqty{g\pqty{x}}}
		=\pqty{\lim\limits_{h\to 0}
		\frac{f\pqty{g+\epsilon}-f\pqty{g}}{\epsilon}:g\to g\pqty{x}}
		\pdiff{x}{}{g\pqty{x}}
		\end{equation}
		Simplify \eqref{DerivLimit}
		\begin{equation}
		\pdiff{x}{}{f\pqty{g\pqty{x}}}
		=\pqty{\pdiff{g}{}f\pqty{g}:g\to g\pqty{x}}
		\pdiff{x}{}{g\pqty{x}}
		\end{equation}
	\end{proof}
	
	\section{Logarithmic Derivative}
	\begin{theorem}
		\begin{equation}
		\label{LogDiff}
		\pdiff{x}{}f\pqty{x}=f\pqty{x}\pdiff{x}{}\ln\pqty{f\pqty{x}}
		\end{equation}
	\end{theorem}
	\begin{proof}
		Use the chain rule
		\begin{equation}
		\pdiff{x}{}\ln\pqty{f\pqty{x}}=
		\pqty{\pdiff{z}{}\ln\pqty{z}:z\to f\pqty{x}}*\pdiff{x}{}{f\pqty{x}}
		\end{equation}
		Simplify. [Logarithms\eqref{LnIntegralForm}]
		\begin{equation}
		\pdiff{x}{}\ln\pqty{f\pqty{x}}=
		\pqty{\frac{1}{z}:z\to f\pqty{x}}*\pdiff{x}{}{f\pqty{x}}=
		\frac{1}{f\pqty{x}}*\pdiff{x}{}{f\pqty{x}}
		\end{equation}
		Multiply
		\begin{equation}
		f\pqty{x}\pdiff{x}{}\ln\pqty{f\pqty{x}}=
		\pdiff{x}{}{f\pqty{x}}
		\end{equation}
	\end{proof}

	\section{Product Rule}
	\begin{theorem}
		\begin{equation}
			\pdiff{x}{}\prod_{k=1}^{n}f\pqty{x}=
			\pqty{\prod_{k=1}^{n}f\pqty{x}}
			\sum_{k=1}^{n}\frac{\pdiff{x}{}f\pqty{x}}{f\pqty{x}}
		\end{equation}
	\end{theorem}
	\begin{proof}
		Use \eqref{LogDiff}
		\begin{equation}
		\pdiff{x}{}\prod_{k=1}^{n}f\pqty{x}=
		\pqty{\prod_{k=1}^{n}f\pqty{x}}\pdiff{x}{}\ln\pqty{\prod_{k=1}^{n}f\pqty{x}}
		\end{equation}
		Expand the logarithms
		\begin{equation}
		\pdiff{x}{}\prod_{k=1}^{n}f\pqty{x}=
		\pqty{\prod_{k=1}^{n}f\pqty{x}}
		\pdiff{x}{}\pqty{\sum_{k=1}^{n}\ln\pqty{f\pqty{x}}}
		\end{equation}
		Sum rule \eqref{DiffSum}
		\begin{equation}
		\pdiff{x}{}\prod_{k=1}^{n}f\pqty{x}=
		\pqty{\prod_{k=1}^{n}f\pqty{x}}
		\pqty{\sum_{k=1}^{n}\pdiff{x}{}\ln\pqty{f\pqty{x}}}
		\end{equation}
		Simplify logarithmic derivative using \eqref{LogDiff}
		\begin{equation}
		\pdiff{x}{}\prod_{k=1}^{n}f\pqty{x}=
		\pqty{\prod_{k=1}^{n}f\pqty{x}}
		{\sum_{k=1}^{n}\frac{\pdiff{x}{}f\pqty{x}}{f\pqty{x}}}
		\end{equation}
	\end{proof}

\end{document}
