\input{NazgandStyle}
\title{
	1 With Varying Base Digits
}
\begin{document}
	
	\maketitle
	
	Let exist a sequence \(a_k\in\mathbb{Z},a_k>1\). Then
	\begin{equation}
		1=\sum_{k\in\mathbb{Z}_{>0}}\frac{a_k-1}{\prod_{m=1}^{k}a_m}
		=\sum_{k=1}^{\infty}\frac{a_k-1}{\prod_{m=1}^{k}a_m}
	\end{equation}

	This can be seen via the limit \(j\to\infty\) in the following equation.
	\begin{equation}
	1-\prod_{m=1}^{j}a_m^{-1}=
	\sum_{k=1}^{j}\frac{a_k-1}{\prod_{m=1}^{k}a_m}
	\end{equation}
	
	Proof of previous equation by induction: For the base case, \(j=0\), we have \(1-1=0\).
	For the inductive step, we can simply prove
	\begin{equation}
		\pqty{1-\prod_{m=1}^{j+1}a_m^{-1}}-\pqty{1-\prod_{m=1}^{j}a_m^{-1}}=
		\pqty{\sum_{k=1}^{j+1}\frac{a_k-1}{\prod_{m=1}^{k}a_m}}-
		\pqty{\sum_{k=1}^{j}\frac{a_k-1}{\prod_{m=1}^{k}a_m}}
	\end{equation}
	
	Simplify both sides to get:
	\begin{equation}
		\prod_{m=1}^{j}a_m^{-1}-\prod_{m=1}^{j+1}a_m^{-1}
		=\sum_{k=j+1}^{j+1}\frac{a_k-1}{\prod_{m=1}^{k}a_m}
		=\frac{a_{j+1}-1}{\prod_{m=1}^{j+1}a_m}
	\end{equation}

	Multiply both sides by \(\prod_{m=1}^{j+1}a_m\):
	\begin{equation}
		a_{j+1}-1=a_{j+1}-1
	\end{equation}
	\qed

\end{document}
