\input{NazgandStyle}
\title{
	Argument Sum Rules From
	
	Homogeneous Linear Differential Equations Of Constant Coefficients
}
\begin{document}
	
	\maketitle
	
	\begin{abstract}
		The goal of this paper is to describe a theorem (previously a conjecture).
	\end{abstract}
	
	\section{Assumptions and definitions}
	A [homogeneous linear differential equation of constant coefficients] has the form
	\begin{equation}
		0=\sum_{k=0}^{n}a_k\pdiff{z}{k}f\pqty{z}
		=\sum_{k=0}^{n}a_k f^\pqty{k}\pqty{z}
	\end{equation}
	where \(\forall k, a_k\in\mathbb{C}\inlineeqnum\), \(n\in\mathbb{Z}_{\geq 0}\inlineeqnum\), \(a_n \neq 0\inlineeqnum\). Let \(f : \mathbb{C}\to\mathbb{C}\inlineeqnum\) be differentiable at least \(n\) times everywhere.
	
	Every [homogeneous linear differential equation of constant coefficients] has at least 1 basis for the vector space of its solutions.
	
	Let \(g_0\pqty{z},\dots,g_{n-1}\pqty{z}\) be such a basis. To be clear:
	\begin{equation}
		\label{BasisExistsForSolutionSet}
		\text{Solutions}=
		\Bqty{h\pqty{z} \mid 0=\sum_{k=0}^{n}a_k h^\pqty{k}\pqty{z}}
		=\Bqty{\sum_{k=0}^{n-1}b_k g_k\pqty{z} \mid b_k\in\mathbb{C}}
	\end{equation}
	Let us define a column vector and clarify its transpose (a row vector):
	\begin{equation}
		v\pqty{z_0}=
		\begin{pmatrix}
			g_0\pqty{z_0} \\
			\vdots \\
			g_{n-1}\pqty{z_0} \\
		\end{pmatrix}
		,
		v\pqty{z_1}\transpose=
		\begin{pmatrix}
			g_0\pqty{z_1} &
			\dots &
			g_{n-1}\pqty{z_1}
		\end{pmatrix}
	\end{equation}
	
	\section{Main theorem with 2 arguments}
	There exists a unique symmetric \(n\) by \(n\) matrix \(A\) (\(A=A\transpose\)) such that
	\begin{equation}
		\label{ArgumentSumRuleMatrix}
		f\pqty{z_0+z_1}=v\pqty{z_1}\transpose A v\pqty{z_0}=v\pqty{z_0}\transpose A v\pqty{z_1}
	\end{equation}
	
	\subsection{A reason \(A\) is symmetric}
	Suppose instead of a symmetric matrix \(A\), we find a matrix \(B\) such that
	\begin{equation}
		f\pqty{z_0+z_1}=v\pqty{z_1}\transpose B v\pqty{z_0}
	\end{equation}
	Then take the transpose of the equation and substitute \(z_0\to z_1,z_1\to z_0\), resulting in the following equation:
	\begin{equation}
		f\pqty{z_0+z_1}=v\pqty{z_1}\transpose B\transpose v\pqty{z_0}
	\end{equation}
	Average both equations:
	\begin{equation}
		f\pqty{z_0+z_1}=v\pqty{z_1}\transpose \frac{B+B\transpose}{2} v\pqty{z_0}
	\end{equation}
	Note that we can set \(A=\frac{B+B\transpose}{2}\) because it is symmetric. \qed
	
	\section{Theorem generalized to positive integer amounts of arguments in addition to 2}
	The following statements use the same assumptions and definitions as the main theorem.
	\subsection{1 argument}
	The following statement, which I call \(\text{ArgSumCon}\pqty{1}\), is trivial by assumption the \(\eqref{BasisExistsForSolutionSet}\).
	\begin{equation}
		\exists! c\pqty{k_0}\in\mathbb{C}, f\pqty{z_0} = \sum_{k_0=0}^{n-1}c\pqty{k_0} g_{k_0}\pqty{z_0}
	\end{equation}
	
	\subsection{2 arguments}
	The following statement, which I call \(\text{ArgSumCon}\pqty{2}\), is equivalent to \(\eqref{ArgumentSumRuleMatrix}\).
	\begin{equation}
		\exists! c\pqty{k_0,k_1}\in\mathbb{C}, f\pqty{z_0+z_1} = \sum_{k_0=0}^{n-1}\sum_{k_1=0}^{n-1}c\pqty{k_0,k_1} g_{k_0}\pqty{z_0} g_{k_1}\pqty{z_1}
	\end{equation}
	
	\subsection{3 arguments}
	The following statement, I call \(\text{ArgSumCon}\pqty{3}\).
	\begin{equation}
		\exists! c\pqty{k_0,k_1,k_2}\in\mathbb{C}, f\pqty{z_0+z_1+z_2} =
		\sum_{k_0=0}^{n-1}\sum_{k_1=0}^{n-1}\sum_{k_2=0}^{n-1}c\pqty{k_0,k_1,k_2} g_{k_0}\pqty{z_0} g_{k_1}\pqty{z_1} g_{k_2}\pqty{z_2}
	\end{equation}
	
	\subsection{\(m\) arguments for \(m\in\mathbb{Z}_{>0}\)}
	The following statement, I call \(\text{ArgSumCon}\pqty{m}\).
	\begin{equation}
		\exists! c\pqty{k_0,k_1,\dots,k_{m-1}}\in\mathbb{C}, f\pqty{\sum_{j=0}^{m-1}z_j} =
		\sum_{k_0=0}^{n-1}\sum_{k_1=0}^{n-1}\dots\sum_{k_{m-1}=0}^{n-1}c\pqty{k_0,k_1,\dots,k_{m-1}} \prod_{j=0}^{m-1}g_{k_j}\pqty{z_j}
	\end{equation}
	Note \(\text{ArgSumCon}\pqty{m+1}\Rightarrow\text{ArgSumCon}\pqty{m}\), as can be seen by replacing 1 of the variables with 0.
	
	\section{Lean 4 code}
	\(\text{ArgSumCon}\pqty{m}\) has been formally proved in and verified by Lean 4:
	
	\href{https://GitHub.Com/Nazgand/NazgandLean4/blob/master/NazgandLean4/HomogeneousLinearDifferentialEquationsOfConstantCoefficients/ArgumentSumRule.lean}
	{https://GitHub.Com/Nazgand/NazgandLean4/blob/master/NazgandLean4/\\HomogeneousLinearDifferentialEquationsOfConstantCoefficients/ArgumentSumRule.lean}
	
	Also verified by Lean 4: the relevant tensor is unique and symmetric.
\end{document}
