\input{../NazgandStyle}
\title{
	Differentiation
}
\begin{document}
	
	\maketitle
	
	\section{Definition}
	\begin{equation}
	\label{DerivLimit}
	\pdiff{x}{}f\pqty{x}=\lim\limits_{h\to 0}\frac{f\pqty{x+h}-f\pqty{x}}{h}
	\end{equation}
	
	\section{Sum Rule}
	\begin{theorem}
		\begin{equation}
		\label{DiffSum}
		\pdiff{x}{}\pqty{f\pqty{x}+g\pqty{x}}=
		\pqty{\pdiff{x}{}f\pqty{x}}+
		\pqty{\pdiff{x}{}g\pqty{x}}
		\end{equation}
		\begin{proof}
			Use \eqref{DerivLimit}
			\begin{equation}
			\pdiff{x}{}\pqty{f\pqty{x}+g\pqty{x}}
			=\lim\limits_{h\to 0}
			\frac{\pqty{f\pqty{x+h}+g\pqty{x+h}}-\pqty{f\pqty{x}+g\pqty{x}}}{h}
			\end{equation}
			Rearrange
			\begin{equation}
			\pdiff{x}{}\pqty{f\pqty{x}+g\pqty{x}}
			=\lim\limits_{h\to 0}
			\pqty{\frac{{f\pqty{x+h}-f\pqty{x}}}{h}
			+
			\frac{{g\pqty{x+h}-g\pqty{x}}}{h}}
			\end{equation}
			Split the limit
			\begin{equation}
			\pdiff{x}{}\pqty{f\pqty{x}+g\pqty{x}}
			=\pqty{\lim\limits_{h\to 0}
			\frac{{f\pqty{x+h}-f\pqty{x}}}{h}}
				+ \pqty{\lim\limits_{a\to 0}
				\frac{{g\pqty{x+a}-g\pqty{x}}}{a}}
			\end{equation}
			Simplify with \eqref{DerivLimit}
			\begin{equation}
			\pdiff{x}{}\pqty{f\pqty{x}+g\pqty{x}}=
			\pqty{\pdiff{x}{}f\pqty{x}}+
			\pqty{\pdiff{x}{}g\pqty{x}}
			\end{equation}
		\end{proof}
	\end{theorem}

	\section{Constant Multiple Rule}
	\begin{theorem}
		\begin{equation}
			\pdiff{x}{}\pqty{a*f\pqty{x}}=
			a*\pdiff{x}{}\pqty{f\pqty{x}}
		\end{equation}
		\begin{proof}
			Use \eqref{DerivLimit}
			\begin{equation}
			\pdiff{x}{}\pqty{a*f\pqty{x}}=
			\lim\limits_{h\to 0}\frac{a*f\pqty{x+h}-a*f\pqty{x}}{h}=
			a*\lim\limits_{h\to 0}\frac{f\pqty{x+h}-f\pqty{x}}{h}=
			a*\pdiff{x}{}\pqty{f\pqty{x}}
			\end{equation}
		\end{proof}
	\end{theorem}

	\section{Chain Rule}
	\begin{theorem}
		\begin{equation}
		\label{DiffChainRule}
		\pdiff{x}{}{f\pqty{g\pqty{x}}}
		=\pqty{\pdiff{g}{}f\pqty{g}\replace{g}{g\pqty{x}}}*\pdiff{x}{}{g\pqty{x}}
		\end{equation}
		\begin{proof}
			Start with \eqref{DerivLimit}
			\begin{equation}
			\pdiff{x}{}{f\pqty{g\pqty{x}}}
			=\lim\limits_{h\to 0}
			\frac{f\pqty{g\pqty{x+h}}-f\pqty{g\pqty{x}}}{h}
			\end{equation}
			Multiply by \(1=\frac{g\pqty{x+h}-g\pqty{x}}{g\pqty{x+h}-g\pqty{x}}\):
			\begin{equation}
			\pdiff{x}{}{f\pqty{g\pqty{x}}}
			=\lim\limits_{h\to 0}
			\frac{f\pqty{g\pqty{x+h}}-f\pqty{g\pqty{x}}}{g\pqty{x+h}-g\pqty{x}}
			\frac{g\pqty{x+h}-g\pqty{x}}{h}
			\end{equation}
			Split the limit:
			\begin{equation}
			\pdiff{x}{}{f\pqty{g\pqty{x}}}
			=\lim\limits_{h\to 0}
			\frac{f\pqty{g\pqty{x+h}}-f\pqty{g\pqty{x}}}{g\pqty{x+h}-g\pqty{x}}
			\lim\limits_{a\to 0}
			\frac{g\pqty{x+a}-g\pqty{x}}{a}
			\end{equation}
			Simplify \eqref{DerivLimit}
			\begin{equation}
			\pdiff{x}{}{f\pqty{g\pqty{x}}}
			=\lim\limits_{h\to 0}
			\frac{f\pqty{g\pqty{x+h}}-f\pqty{g\pqty{x}}}{g\pqty{x+h}-g\pqty{x}}
			\pdiff{x}{}{g\pqty{x}}
			\end{equation}
			Substitute \(g\pqty{x+h}\to g+\epsilon,g\pqty{x}\to g\)
			\begin{equation}
			\pdiff{x}{}{f\pqty{g\pqty{x}}}
			=\pqty{\lim\limits_{\epsilon\to 0}
			\frac{f\pqty{g+\epsilon}-f\pqty{g}}{\epsilon}\replace{g}{g\pqty{x}}}
			\pdiff{x}{}{g\pqty{x}}
			\end{equation}
			Simplify \eqref{DerivLimit}
			\begin{equation}
			\pdiff{x}{}{f\pqty{g\pqty{x}}}
			=\pqty{\pdiff{g}{}f\pqty{g}\replace{g}{g\pqty{x}}}
			\pdiff{x}{}{g\pqty{x}}
			\end{equation}
		\end{proof}
	\end{theorem}
	
	\section{Logarithmic Derivative}
	\begin{theorem}
		\begin{equation}
		\label{LogDiff}
		\pdiff{x}{}f\pqty{x}=f\pqty{x}\pdiff{x}{}\ln\pqty{f\pqty{x}}
		\end{equation}
		\begin{proof}
			Use the chain rule
			\begin{equation}
			\pdiff{x}{}\ln\pqty{f\pqty{x}}=
			\pqty{\pdiff{z}{}\ln\pqty{z}\replace{z}{f\pqty{x}}}*\pdiff{x}{}{f\pqty{x}}
			\end{equation}
			Simplify. [Logarithms\eqref{LnIntegralForm}]
			\begin{equation}
			\pdiff{x}{}\ln\pqty{f\pqty{x}}=
			\pqty{\frac{1}{z}\replace{z}{f\pqty{x}}}*\pdiff{x}{}{f\pqty{x}}=
			\frac{1}{f\pqty{x}}*\pdiff{x}{}{f\pqty{x}}
			\end{equation}
			Multiply
			\begin{equation}
			f\pqty{x}\pdiff{x}{}\ln\pqty{f\pqty{x}}=
			\pdiff{x}{}{f\pqty{x}}
			\end{equation}
		\end{proof}
	\end{theorem}

	\section{Product Rule}
	\begin{theorem}
		\begin{equation}
			\pdiff{x}{}\prod_{k=1}^{n}f_k\pqty{x}=
			\pqty{\prod_{k=1}^{n}f_k\pqty{x}}
			\sum_{k=1}^{n}\frac{\pdiff{x}{}f_k\pqty{x}}{f_k\pqty{x}}
		\end{equation}
		\begin{proof}
			Use \eqref{LogDiff}
			\begin{equation}
			\pdiff{x}{}\prod_{k=1}^{n}f_k\pqty{x}=
			\pqty{\prod_{k=1}^{n}f_k\pqty{x}}\pdiff{x}{}\ln\pqty{\prod_{k=1}^{n}f_k\pqty{x}}
			\end{equation}
			Expand the logarithms
			\begin{equation}
			\pdiff{x}{}\prod_{k=1}^{n}f_k\pqty{x}=
			\pqty{\prod_{k=1}^{n}f_k\pqty{x}}
			\pdiff{x}{}\pqty{\sum_{k=1}^{n}\ln\pqty{f_k\pqty{x}}}
			\end{equation}
			Sum rule \eqref{DiffSum}
			\begin{equation}
			\pdiff{x}{}\prod_{k=1}^{n}f_k\pqty{x}=
			\pqty{\prod_{k=1}^{n}f_k\pqty{x}}
			\pqty{\sum_{k=1}^{n}\pdiff{x}{}\ln\pqty{f_k\pqty{x}}}
			\end{equation}
			Simplify logarithmic derivative using \eqref{LogDiff}
			\begin{equation}
			\pdiff{x}{}\prod_{k=1}^{n}f_k\pqty{x}=
			\pqty{\prod_{k=1}^{n}f_k\pqty{x}}
			{\sum_{k=1}^{n}\frac{\pdiff{x}{}f_k\pqty{x}}{f_k\pqty{x}}}
			\end{equation}
		\end{proof}
	\end{theorem}

\end{document}
