\input{../NazgandStyle}
\title{
	Logarithms
}
\begin{document}
	
	\maketitle
	
	\section{Logarithms}
	\begin{definition}
		The logarithm functions are the inverse functions of the exponentiation functions:
		\begin{equation}
			\label{LogarithmDefinition}
			\bqty{\Bqty{b,x}\subset\mathbb{C}\land b\ne 0}\Rightarrow
			b^{\log_b\pqty{x}}=x
		\end{equation}
		\begin{equation}
			\label{RealLogarithmSimp}
			\bqty{\Bqty{b,x}\subset\mathbb{R}\land b>0}\Rightarrow
			\log_b\pqty{b^x}=x
		\end{equation}
		\begin{equation}
		\log_e\pqty{x}=\ln\pqty{x}
		\end{equation}
	\end{definition}

	\begin{theorem}[Power rule]
		\begin{equation}
			\bqty{\Bqty{b,x}\subset\mathbb{R}\land b>0}\Rightarrow		\log_b\pqty{x^p}=p*\log_b\pqty{x}
		\end{equation}
		\begin{proof}
			Start with \eqref{LogarithmDefinition}:
			\begin{equation}
			b^{\log_b\pqty{x}}=x
			\end{equation}
			Raise both sides to the power of \(p\):
			\begin{equation}
			b^{p*\log_b\pqty{x}}=x^p
			\end{equation}
			Apply the \(\log_b\) function to both sides, simplifying with \eqref{RealLogarithmSimp}:
			\begin{equation}
			p*\log_b\pqty{x}=\log_b\pqty{x^p}
			\end{equation}
		\end{proof}
	\end{theorem}

	\begin{theorem}[Product sum rule]
		\begin{equation}
		\log_b\pqty{x*y}=\log_b\pqty{x}+\log_b\pqty{y}
		\end{equation}
		\begin{proof}
			Use \eqref{LogarithmDefinition}
			\begin{equation}
			\log_b\pqty{x*y}=
			\log_b\pqty{b^{\log_b\pqty{x}}*b^{\log_b\pqty{x}}}
			\end{equation}
			Use the additive property of exponential functions
			\begin{equation}
			\log_b\pqty{x*y}=
			\log_b\pqty{b^{\log_b\pqty{x}+\log_b\pqty{x}}}
			\end{equation}
			Use \eqref{LogarithmDefinition}
			\begin{equation}
			\log_b\pqty{x*y}=
			\log_b\pqty{x}+\log_b\pqty{x}
			\end{equation}
		\end{proof}
	\end{theorem}

	\begin{theorem}[Change of base]
		\begin{equation}
			\log_b\pqty{x}=\frac{\log_k\pqty{x}}{\log_k\pqty{b}}
		\end{equation}
		\begin{proof}
			Start with \eqref{LogarithmDefinition}:
			\begin{equation}
				b^{\log_b\pqty{x}}=x
			\end{equation}
			Apply the \(\log_k\) function to both sides:
			\begin{equation}
				\log_k\pqty{b^{\log_b\pqty{x}}}=\log_k\pqty{x}
			\end{equation}
			\begin{equation}
				\log_b\pqty{x}\log_k\pqty{b}=\log_k\pqty{x}
			\end{equation}
			Divide both sides by \(\log_k\pqty{b}\)
		\end{proof}
	\end{theorem}

	\begin{theorem}[Integral form]
		\begin{equation}
		\label{LnIntegralForm}
		z\in\mathbb{R}^+\Rightarrow
		\ln\pqty{z}=\dint{1}{z}{\frac{1}{x}}{x}
		\end{equation}
	\begin{proof}
		Proof from \url{https://math.stackexchange.com/q/1341995}. 
		The derivative of the logarithm functions exist because the exponential functions have derivatives.
		\url{https://en.wikipedia.org/wiki/Inverse_function_theorem}
		\begin{equation}
		\pdiff{x}{}x=1
		\end{equation}
		Substitute \eqref{LogarithmDefinition}:
		\begin{equation}
		\pdiff{x}{}e^{\ln\pqty{x}}=1
		\end{equation}
		The chain rule [Differentiation\eqref{DiffChainRule}]
		\begin{equation}
		\pqty{\pdiff{z}{}e^{z}\replace{z}{\ln\pqty{x}}}\pdiff{x}{}{\ln\pqty{x}}=1
		\end{equation}
		The derivative of the natural exponential function is itself: [ExponentialFunction\eqref{expOwnDeriv}]
		\begin{equation}
		\pqty{e^{z}\replace{z}{\ln\pqty{x}}}\pdiff{x}{}{\ln\pqty{x}}=1
		\end{equation}
		Substitute:
		\begin{equation}
		e^{\ln\pqty{x}}\pdiff{x}{}{\ln\pqty{x}}=1
		\end{equation}
		Simplify:
		\begin{equation}
		x\pdiff{x}{}{\ln\pqty{x}}=1
		\end{equation}
		Divide:
		\begin{equation}
		\pdiff{x}{}{\ln\pqty{x}}=\frac{1}{x}
		\end{equation}
		Integrate:
		\begin{equation}
		\ln\pqty{z}={\ln\pqty{z}-\ln\pqty{1}}=\dint{1}{z}{\frac{1}{x}}{x}
		\end{equation}
		
	\end{proof}
	\end{theorem}


	
	
	\url{https://en.wikipedia.org/wiki/Logarithm}
\end{document}
